formal/IO.thy
@@ -24,10 +24,33 @@ definition blankips :: "inputs" where
 "blankips \<equiv> \<lambda>x . None"
 declare blankips_def [simp]
 
+definition set_reg :: "dataname \<Rightarrow> valuetype option \<Rightarrow> data" where
+"set_reg n v \<equiv> (\<lambda>k . if k = n then v else None)"
+
 (* Stuff for making traces from simpler to type stuff... *)
-definition overwrite :: "('a \<Rightarrow> 'b) \<Rightarrow> ('a * 'b) \<Rightarrow> ('a \<Rightarrow> 'b)" (infix "\<oplus>" 50) where
-"overwrite \<equiv> \<lambda>f . \<lambda>(k,v) . \<lambda>kk . if kk = k then v else f(kk)"
+definition overwrite :: "('a \<Rightarrow> 'b option) \<Rightarrow> ('a \<Rightarrow> 'b option) \<Rightarrow> ('a \<Rightarrow> 'b option)" (infix "\<oplus>" 50) where
+"overwrite \<equiv> \<lambda>f . \<lambda>g . \<lambda>kk . 
+  case g(kk) of
+    None \<Rightarrow> f(kk)
+    | Some v \<Rightarrow> Some v"
 declare overwrite_def[simp]
+
+definition make_update :: "dataname => exp => updates" ("r _/ := _/" 50) where
+"(r n := e) \<equiv> \<lambda>(dt,ip) . dt \<oplus> (set_reg n (eval (dt,ip) e))"
+
+fun make_updates :: "updates list \<Rightarrow> updates" ("u _" 50) where
+"u [] = noupdates"
+| "u (a#as) = (\<lambda>(dt,ip) . ((u as)(dt,ip)) \<oplus> (a(dt,ip)))"
+
+value "((u [r 1 := (Lit (In 1)), r 2 := (Lit (In 4))])(blankdata,blankips))(1)"
+
+lemma overwriting:
+  fixes n
+  shows "u [r n := v, r n := vv] \<equiv> r n := vv"
+  apply (simp only: make_updates.simps)
+
+lemma noupdates_left_id : "u [noupdates, x] \<equiv> u [x]"
+  
 
 primrec make_trace_step :: "inputs \<Rightarrow> valuetype list => int \<Rightarrow> inputs" where
 "make_trace_step ips [] _ = ips"
