formal/Lift.thy
@@ -1,0 +1,7 @@
+theory Lift
+  imports EFSM
+begin
+
+
+
+end
