formal/Types.thy
@@ -8,11 +8,12 @@ type_synonym outputname = int
 type_synonym label = string
 type_synonym arity = int
 
-type_synonym valuetype = "(int + string)"
+datatype valuetype = In int | St string
+datatype exp = Lit valuetype | R dataname | I inputname | Plus exp exp | Minus exp exp | Mul exp exp
 
-type_synonym inputs = "inputname \<Rightarrow> valuetype option"
-type_synonym data = "dataname \<Rightarrow> valuetype option"
-type_synonym outvalues = "outputname \<Rightarrow> valuetype option"
+type_synonym inputs = "(inputname, valuetype) map"
+type_synonym data = "(dataname, valuetype) map"
+type_synonym outvalues = "(outputname, valuetype) map"
 
 type_synonym guard = "(inputs \<times> data) => bool"
 type_synonym outputs = "(inputs \<times> data) => outvalues"
@@ -30,7 +31,7 @@ type_synonym statename = "int"
 record efsm =
   S :: "statename list"
   s0 :: "statename"
-  M :: "(statename * statename) \<Rightarrow> transition list"
+  M :: "((statename * statename), transition list) map"
 
 type_synonym trace = "(label \<times> inputs) list"
 type_synonym observation = "outvalues list"
@@ -38,16 +39,18 @@ type_synonym observation = "outvalues list"
 (* This now treats None as 0. 
 This isn't ideal but it means that we don't have to pre-initialise variables *)
 fun MaybeApplyInt :: "(int \<Rightarrow> int \<Rightarrow> int) \<Rightarrow> valuetype option \<Rightarrow> valuetype option \<Rightarrow> valuetype option" where
-"MaybeApplyInt f None None = Some (Inl (f 0 0))"
+(* "MaybeApplyInt f None None = Some (Inl (f 0 0))"
 |"MaybeApplyInt f None (Some (Inl r)) = (Some (Inl (f 0 r)))"
-|"MaybeApplyInt f (Some (Inl l)) None= (Some (Inl (f l 0)))"
-|"MaybeApplyInt f (Some (Inl a)) (Some (Inl b)) = Some (Inl (f a b))"
+|"MaybeApplyInt f (Some (Inl l)) None = (Some (Inl (f l 0)))" *)
+"MaybeApplyInt f _ None = None"
+|"MaybeApplyInt f None _ = None"
+|"MaybeApplyInt f (Some (In a)) (Some (In b)) = Some (In (f a b))"
 |"MaybeApplyInt _ _ _ = None"
 
 fun MaybeBoolInt :: "(int \<Rightarrow> int \<Rightarrow> bool) \<Rightarrow> valuetype option \<Rightarrow> valuetype option \<Rightarrow> bool" where
 "MaybeBoolInt _ None _ = False"
 |"MaybeBoolInt _ _ None = False"
-|"MaybeBoolInt f (Some (Inl a)) (Some (Inl b)) = (f a b)"
+|"MaybeBoolInt f (Some (In a)) (Some (In b)) = (f a b)"
 |"MaybeBoolInt _ _ _ = False"
 
 abbreviation MaybePlus :: "valuetype option \<Rightarrow> valuetype option \<Rightarrow> valuetype option" (infix "+" 40) where
@@ -56,6 +59,14 @@ abbreviation MaybeMinus :: "valuetype option \<Rightarrow> valuetype option \<Ri
 "a - b \<equiv> MaybeApplyInt (\<lambda>x::int.\<lambda>y::int.(x-y)) a b"
 abbreviation MaybeMul :: "valuetype option \<Rightarrow> valuetype option \<Rightarrow> valuetype option" (infix "*" 40) where
 "a * b \<equiv> MaybeApplyInt (\<lambda>x::int.\<lambda>y::int.(x*y)) a b"
+
+fun eval :: "data \<times> inputs \<Rightarrow> exp \<Rightarrow> valuetype option" where
+"eval _ (Lit v) = Some v"
+|"eval (dt,_) (R n) = dt(n)"
+|"eval (_,ip) (I n) = ip(n)"
+|"eval ctx (Plus e1 e2) = MaybePlus (eval ctx e1) (eval ctx e2)"
+|"eval ctx (Minus e1 e2) = MaybeMinus (eval ctx e1) (eval ctx e2)"
+|"eval ctx (Mul e1 e2) = MaybeMul (eval ctx e1) (eval ctx e2)"
 
 abbreviation MaybeGt :: "valuetype option \<Rightarrow> valuetype option \<Rightarrow> bool" (infix ">" 40) where
 "a > b \<equiv> MaybeBoolInt (\<lambda>x::int.\<lambda>y::int.(x>y)) a b"
